Especificaciones/Auxiliar/MultisetFacts.dfy
@@ -1,0 +1,113 @@
+lemma CommutativeUnion<T>(x:multiset<T>,y:multiset<T>)
+ensures x + y == y + x
+{}
+
+lemma AssociativeUnion<T>(x:multiset<T>,y:multiset<T>,z:multiset<T>)
+ensures x + (y + z) == (x + y) + z
+{}
+
+lemma CommutativeAssociativeUnion<T>(x:multiset<T>,y:multiset<T>,z:multiset<T>,u:multiset<T>)
+ensures (x + y) + (z + u) == (x + u) + (y + z)
+{} 
+
+lemma IntersectionContained<T>(A: multiset<T>,B:multiset<T>)
+ensures A * B <= A && A * B <= B
+{}
+
+lemma IntersectionUnion<T>(x:multiset<T>,y:multiset<T>,z:multiset<T>)
+requires  z >=  x + y
+ensures (x + y) * z == (x * z + y * z)
+{}
+
+lemma IntersectionUnionContained<T>(x:multiset<T>,y:multiset<T>,z:multiset<T>)
+ensures  x * z + y * z >= (x + y) * z
+{}
+
+lemma SubstractUnion<T>(x:multiset<T>,y:multiset<T>)
+requires y >= x
+ensures x + (y - x) == y
+{} 
+
+lemma UnionSubstractUnion<T>(x:multiset<T>,y:multiset<T>,z:multiset<T>,u:multiset<T>)
+requires x + y >= z + u && x >= z && y >= u
+ensures (x + y) - (z + u) == (x - z) + (y - u)
+{}
+
+ghost function Union (I:multiset<multiset<nat>>) : multiset<nat>
+{
+  if I == multiset{} then multiset{}
+  else var i :| i in I; i + Union(I-multiset{i})
+}
+
+lemma UnionOne(C: multiset<multiset<nat>>, P1:multiset<nat>)
+requires P1 in C
+ensures Union(C) == P1 + Union(C-multiset{P1})
+{ 
+    var i:| i in C && Union(C) == i + Union(C-multiset{i});
+    if (i == P1) {
+    }
+    else {
+        
+        calc{
+         Union(C);
+         i + Union(C-multiset{i});
+         {assert P1 in C-multiset{i};
+         UnionOne(C-multiset{i},P1);}
+         i + (P1 + Union(C-multiset{i}-multiset{P1}));
+         {assert C -multiset{i}-multiset{P1} ==  C-multiset{P1}-multiset{i};}
+         P1 + (i + Union(C-multiset{P1}-multiset{i}));
+         {UnionOne(C-multiset{P1},i);}
+         P1 + Union(C-multiset{P1});
+        }
+       
+    }
+
+}
+
+lemma Union2(C: multiset<multiset<nat>>,P1: multiset<nat>, P2: multiset<nat>)
+requires C == multiset{P1,P2}
+ensures Union(C) == P1 + P2
+{
+ UnionOne(C,P1);
+ assert Union(C) == P1 + Union(C-multiset{P1});
+ UnionOne(C-multiset{P1},P2);
+ assert Union(C-multiset{P1}) == Union((C-multiset{P1})-multiset{P2})+ P2;
+ assert (C-multiset{P1})-multiset{P2} == multiset{};
+ assert  Union(C)  == P1 + P2;
+}
+
+
+
+lemma Multiset2(C: multiset<multiset<nat>>)
+requires |C| == 2
+ensures exists P1,P2 :: multiset{P1,P2} == C
+{
+    var P1:multiset<nat> :| P1 in C; 
+    // assert P1 < EA; // P1 = {1,2}
+    var CC := C - multiset{P1};
+    SubstractUnion(multiset{P1},C);
+    assert  CC + multiset{P1} == C ;
+    
+    assert |CC| > 0;
+    var P2:multiset<nat> :| P2 in CC; 
+    var CC' := CC - multiset{P2};
+    SubstractUnion(multiset{P2},CC);
+    assert  CC' + multiset{P2} == CC ;
+    assert CC' == multiset{};
+    assert CC' + multiset{P2} == multiset{P2};
+    assert (CC' + multiset{P2}) + multiset{P1} == multiset{P1,P2};
+    assert (CC' + multiset{P2}) + multiset{P1} == C;
+    assert multiset{P1,P2} == C;
+
+
+}
+
+lemma  Multiset1(C: multiset<multiset<nat>>)
+requires |C| == 1
+ensures exists P1 :: multiset{P1} == C
+{ var P1:multiset<nat> :| P1 in C; 
+    // assert P1 < EA; // P1 = {1,2}
+    var CC := C - multiset{P1};
+    SubstractUnion(multiset{P1},C);
+    assert  CC + multiset{P1} == C ;
+}
