Especificaciones/Auxiliar/Sum.dfy
@@ -1,0 +1,240 @@
+function minNat(m:multiset<nat>): (l:nat)
+requires m != multiset{}
+ensures l in m && (forall x | x in m :: l <= x) 
+{ minInt(m)
+}
+
+function minInt(m:multiset<int>): (l:int)
+requires m != multiset{}
+ensures l in m && (forall x | x in m :: l <= x) 
+{ HasMinimumInt(m);
+  var x :| x in m && (forall y | y in m :: x <= y); 
+  x
+}
+
+
+
+
+lemma HasMinimumInt(m: multiset<int>)
+  requires m != multiset{}
+  ensures exists z :: z in m && forall y | y in m :: z <= y
+{
+  var z :| z in m;
+  if m == multiset{z} {
+    // the mimimum of a singleton set is its only element
+  } else if forall y :: y in m ==> z <= y {
+    // we happened to pick the minimum of s
+  } else {
+    // s-{z} is a smaller, nonempty set and it has a minimum
+    var m' := m - multiset{z};
+    HasMinimumInt(m');
+    var z' :| z' in m' && forall y :: y in m' ==> z' <= y;
+    // the minimum of s' is the same as the miminum of s
+    forall y | y in m
+      ensures z' <= y
+    {
+      if
+      case y in m' =>
+        assert z' <= y;  // because z' in minimum in s'
+      case y == z =>
+        var k :| k in m && k < z;  // because z is not minimum in s
+        assert k in m';  // because k != z
+    }
+  }
+}
+
+function FSumNat(m : multiset<nat>) : nat
+{ 
+  if m == multiset{} then 0 
+  else 
+  var x := minNat(m);
+  x + FSumNat(m - multiset{x})
+}
+
+function FSumInt(m : multiset<int>) : int
+{ 
+  if m == multiset{} then 0 
+  else 
+   var x := minInt(m);
+   x + FSumInt(m - multiset{x})
+}
+
+ghost function GSumInt(m: multiset<int>) : int
+{
+  if m == multiset{} then 0
+  else var x :| x in m; x + GSumInt(m - multiset{x})
+}
+
+ghost function GSumNat(m: multiset<nat>) : nat
+{
+  if m == multiset{} then 0
+  else var x :| x in m; x + GSumNat(m - multiset{x})
+}
+
+lemma {:induction m} FSumNatComputaGSumNat(m : multiset<nat>)
+ensures FSumNat(m) == GSumNat(m)
+{ //reveal GSumNat();
+  if m == multiset{} 
+  {
+   // assert GSumNat(m) == 0;
+  }
+  else
+  {
+    var x := minNat(m);
+  //  assert FSumNat(m) == x + FSumNat(m - multiset{x});
+    FSumNatComputaGSumNat(m - multiset{x});
+   // assert FSumNat(m - multiset{x}) == GSumNat(m - multiset{x});
+    GSumNatPartes(m, multiset{x}, m - multiset{x});
+   // assert x + GSumNat(m - multiset{x}) == GSumNat(m);
+  }
+}
+
+lemma {:induction m} FSumIntComputaGSumInt(m : multiset<int>)
+ensures FSumInt(m) == GSumInt(m)
+{ 
+  if m == multiset{} 
+  {
+   // assert GSumInt(m) == 0;
+  }
+  else
+  {
+    var x := minInt(m);
+    FSumIntComputaGSumInt(m - multiset{x});
+    GSumIntPartes(m, multiset{x}, m - multiset{x});
+  }
+}
+
+
+
+lemma GSumPositiveIntNat(m:multiset<nat>)
+ensures GSumInt(m) == GSumNat(m)
+{ 
+  if m == multiset{} {}
+  else {
+    var x:| x in m && GSumNat(m) == x + GSumNat(m - multiset{x});
+    GSumPositiveIntNat(m - multiset{x});
+    GSumIntElemIn(m, x);   
+  }
+}
+
+
+
+
+lemma GSumNatPartes(A:multiset<nat>, P1:multiset<nat>, P2:multiset<nat>)
+    requires P1 <= A && P2 <= A && P1 + P2 == A 
+    ensures GSumNat(A) == GSumNat(P1) + GSumNat(P2)
+  {
+   GSumPositiveIntNat(A);
+   GSumPositiveIntNat(P1);
+   GSumPositiveIntNat(P2);
+   GSumIntPartes(A,P1,P2);
+
+  }
+
+lemma  GSumIntElemIn(A:multiset<int>,i:int)
+requires i in A
+ensures GSumInt(A) == i + GSumInt(A-multiset{i})
+{ 
+  if (A == multiset{}) {}
+  else{
+    var m :| m in A && GSumInt(A) == GSumInt(A-multiset{m}) + m;
+    if (m == i) {}
+    else {
+      GSumIntElemIn(A-multiset{m},i);
+      assert GSumInt(A-multiset{m}) == i + GSumInt(A-multiset{m}-multiset{i});
+      assert GSumInt(A) == i + GSumInt(A-multiset{m}-multiset{i}) + m;
+      GSumIntElemIn(A-multiset{i},m);
+      assert GSumInt(A-multiset{i}) == m + GSumInt(A-multiset{i}-multiset{m});
+      assert A-multiset{i}-multiset{m} == A-multiset{m}-multiset{i};
+      }
+
+  }
+}
+
+
+lemma GSumIntElem(A:multiset<int>, i:int)
+ensures GSumInt(A+multiset{i}) == i + GSumInt(A)
+{ 
+  GSumIntElemIn(A+multiset{i},i);
+  assert A+multiset{i}-multiset{i} == A;
+}
+
+lemma GSumIntPartes(A:multiset<int>, P1:multiset<int>, P2:multiset<int>)
+    requires P1 <= A && P2 <= A && P1 + P2 == A 
+    ensures GSumInt(A) == GSumInt(P1) + GSumInt(P2)
+{ 
+  if (A == multiset{}) {
+    assert P1 == multiset{};
+    assert P2 == multiset{};
+    assert GSumInt(A) == GSumInt(P1) + GSumInt(P2);
+  }
+  else {
+    var i :| i in A;
+    if (i in P1) {
+      // Demostracion 1 : Sum(A-i) == Sum(P1-i) + Sum(P2)  Quitamos i para el paso inductivo
+      GSumIntPartes(A - multiset{i}, P1 - multiset{i}, P2);
+      assert GSumInt(A - multiset{i}) == GSumInt(P1 - multiset{i}) + GSumInt(P2);
+
+      // Demostracion 2 : Sum(A) == i + Sum(A-i) 
+      GSumIntElemIn(A,i);
+      
+      // Demostracion 3 : Sum(P1) == i + Sum(P1-i) 
+      GSumIntElemIn(P1,i);
+
+      assert GSumInt(A) == GSumInt(P1) + GSumInt(P2);
+    }
+    else {
+      GSumIntPartes(A - multiset{i}, P1, P2 - multiset{i});
+      GSumIntElemIn(A,i);
+      GSumIntElemIn(P2,i);         
+    }
+
+  }
+}
+
+
+method {:verify true} mSumaNat(A:multiset<nat>) returns (s:nat)
+ensures s == GSumNat(A)
+{ 
+  var A' := A;
+  s := 0; var e:int; 
+  
+  while |A'| > 0
+  decreases |A'|
+  invariant A' <= A
+  invariant s == GSumNat(A - A')
+   { 
+     e := minInt(A');
+     assert e in A';
+     GSumNatPartes(A - (A'-multiset{e}), A - A',multiset{e});
+     assert s + e == GSumNat(A - (A'-multiset{e}));
+     s := s + e;
+     A' := A' - multiset{e};
+   }
+  assert A' == multiset{} && A - A' == A;
+  assert s == GSumNat(A);
+}
+
+method {:verify true} mSumaInt(A:multiset<int>) returns (s:int)
+ensures s == GSumInt(A)
+{ 
+  var A' := A;
+  s := 0; var e:int; 
+  
+  while |A'| > 0
+  decreases |A'|
+  invariant A' <= A
+  invariant s == GSumInt(A - A')
+   { 
+     e := minInt(A');
+     assert e in A';
+     GSumIntPartes(A - (A'-multiset{e}), A - A',multiset{e});
+     assert s + e == GSumInt(A - (A'-multiset{e}));
+     s := s + e;
+     A' := A' - multiset{e};
+   }
+  assert A' == multiset{} && A - A' == A;
+  assert s == GSumInt(A);
+}
+
+
